Flow/Examples/SimpleProgram.lean
@@ -1,0 +1,69 @@
+import Flow.Lang.Defs
+import Flow.Lang.CFG
+import Flow.Analysis.CP
+import Flow.Lang.BuildSpec
+import Flow.Utils.DotPrinter
+
+open Flow.Analysis Flow.Analysis.CP Flow.Lang Flow.Analysis.Generic
+
+open Expr Stmt BinOp
+
+def simple :=
+  Seq (Decl "a" (.Int 0))
+    (Seq (Decl "b" (.Int 1))
+      (If (BinOp gt (Var "n") (.Int 0))
+        (Assign "b" (BinOp add (Var "a") (Var "b")))
+        (Assign "b" (BinOp add (Var "b") (Var "b")))))
+
+def simpleCFG : CFG :=
+  let (b, (entry, exit)) := CFGBuilder.empty.buildGraph simple
+  { b.cfg with entry, exit }
+
+def sv := varsInProgram simpleCFG
+-- to refactor out: shouldn't need to carry this around
+lemma sv_nodup : sv.Nodup := eraseDups_nodup sv
+
+-- to refactor out: these proofs should work for all CFGs so shouldn't need to
+-- have it around.
+private lemma sv_edges_wf : ∀ {e} {_ : e ∈ simpleCFG.edges},
+  e.src < simpleCFG.nodes.length := by decide
+def sv_CFG := forCFG simpleCFG (by {
+  intro n e he
+  apply sv_edges_wf
+  grind [inEdges]
+})
+
+def res := runDataflow sv_CFG (cpTransfer sv simpleCFG)
+    (cpEdgeTransfer sv)
+    (cpEntryInit sv)
+
+def rd := fun n =>
+    if h : n ∈ sv_CFG.nodes then res.1 ⟨n, h⟩
+    else (fun _ => CPVal.bot)
+
+lemma rd_postfix :
+    PostFixpoint (cpDFA sv) cpAbsorbs simpleCFG rd := by
+  intro n n' hn hn' ⟨k, hedge⟩
+  unfold CFG.hasEdge at hedge
+  simp only [cpAbsorbs]
+  have hedges : simpleCFG.edges =
+      [⟨2,3,.TBranch⟩, ⟨2,4,.FBranch⟩, ⟨3,5,.Normal⟩,
+       ⟨4,5,.Normal⟩, ⟨1,2,.Normal⟩, ⟨0,1,.Normal⟩] := by decide
+  rw [hedges] at hedge
+  clear hedges
+  simp only [List.mem_cons, Edge.mk.injEq, List.not_mem_nil, or_false] at hedge
+  rcases hedge
+    with ⟨rfl,rfl,rfl⟩|⟨rfl,rfl,rfl⟩|⟨rfl,rfl,rfl⟩|⟨rfl,rfl,rfl⟩|⟨rfl,rfl,rfl⟩|⟨rfl,rfl,rfl⟩
+  all_goals native_decide -- sheesh
+
+theorem cp_correct
+    {n n' : Nat}
+    {h : n < simpleCFG.nodes.length} {h' : n' < simpleCFG.nodes.length}
+    {σ σ'}
+    (hsteps : Flow.Eval.Refinement.StepsN simpleCFG h σ h' σ')
+    (hcorr : cpβ_corr simpleCFG (rd n) σ) :
+    cpβ_corr simpleCFG (rd n') σ' :=
+  Flow.Analysis.CP.soundness sv_nodup rd_postfix hsteps hcorr
+
+#eval IO.println (CFG.toDot simpleCFG)
+#eval IO.println (CFG.toDotWith simpleCFG sv_CFG res.1 res.2)
